# baseURI: https://spec.edmcouncil.org/fibo/ontology/master/latest/SEC/Debt/AssetBackedSecurities/PoolBackedSecurities/
# imports: https://spec.edmcouncil.org/fibo/ontology/master/latest/FBC/DebtAndEquities/Debt/
# imports: https://spec.edmcouncil.org/fibo/ontology/master/latest/FBC/FinancialInstruments/FinancialInstruments/
# imports: https://spec.edmcouncil.org/fibo/ontology/master/latest/FND/Accounting/AccountingEquity/
# imports: https://spec.edmcouncil.org/fibo/ontology/master/latest/FND/Agreements/Contracts/
# imports: https://spec.edmcouncil.org/fibo/ontology/master/latest/FND/Arrangements/Arrangements/
# imports: https://spec.edmcouncil.org/fibo/ontology/master/latest/FND/Relations/Relations/
# imports: https://spec.edmcouncil.org/fibo/ontology/master/latest/FND/Utilities/AnnotationVocabulary/
# imports: https://spec.edmcouncil.org/fibo/ontology/master/latest/SEC/Debt/Bonds/
# imports: https://spec.edmcouncil.org/fibo/ontology/master/latest/SEC/Debt/DebtInstruments/
# imports: https://spec.edmcouncil.org/fibo/ontology/master/latest/SEC/Securities/Pools/
# imports: https://spec.edmcouncil.org/fibo/ontology/master/latest/SEC/Securities/SecuritiesIssuance/

@base <https://spec.edmcouncil.org/fibo/ontology/master/latest/SEC/Debt/AssetBackedSecurities/PoolBackedSecurities/> .
@prefix dct: <http://purl.org/dc/terms/> .
@prefix fibo-fbc-dae-dbt: <https://spec.edmcouncil.org/fibo/ontology/FBC/DebtAndEquities/Debt/> .
@prefix fibo-fnd-acc-aeq: <https://spec.edmcouncil.org/fibo/ontology/FND/Accounting/AccountingEquity/> .
@prefix fibo-fnd-agr-ctr: <https://spec.edmcouncil.org/fibo/ontology/FND/Agreements/Contracts/> .
@prefix fibo-fnd-arr-arr: <https://spec.edmcouncil.org/fibo/ontology/FND/Arrangements/Arrangements/> .
@prefix fibo-fnd-rel-rel: <https://spec.edmcouncil.org/fibo/ontology/FND/Relations/Relations/> .
@prefix fibo-fnd-utl-av: <https://spec.edmcouncil.org/fibo/ontology/FND/Utilities/AnnotationVocabulary/> .
@prefix fibo-sec-dbt-ab-pbs: <https://spec.edmcouncil.org/fibo/ontology/SEC/Debt/AssetBackedSecurities/PoolBackedSecurities/> .
@prefix fibo-sec-dbt-dbti: <https://spec.edmcouncil.org/fibo/ontology/SEC/Debt/DebtInstruments/> .
@prefix fibo-sec-sec-iss: <https://spec.edmcouncil.org/fibo/ontology/SEC/Securities/SecuritiesIssuance/> .
@prefix fibo-sec-sec-pls: <https://spec.edmcouncil.org/fibo/ontology/SEC/Securities/Pools/> .
@prefix owl: <http://www.w3.org/2002/07/owl#> .
@prefix rdf: <http://www.w3.org/1999/02/22-rdf-syntax-ns#> .
@prefix rdfs: <http://www.w3.org/2000/01/rdf-schema#> .
@prefix skos: <http://www.w3.org/2004/02/skos/core#> .
@prefix sm: <http://www.omg.org/techprocess/ab/SpecificationMetadata/> .
@prefix xsd: <http://www.w3.org/2001/XMLSchema#> .

<https://spec.edmcouncil.org/fibo/ontology/SEC/Debt/AssetBackedSecurities/PoolBackedSecurities/>
	a owl:Ontology ;
	rdfs:label "Pool-backed Securities Ontology"@en ;
	dct:abstract """Concepts common to asset backed and mortgage backed securities, including pools, instruments, prospectuses and deals common concepts. 
		Note that in common industry parlance, the term 'asset backed security' is used to refer to securities which specifically do not have a mortgage loan pool as their underlying asset. For this reason, this ontology provides a common parent to both asset backed and mortgage backed securities, which is effectively an asset backed security in the broader sense. This has been labeled as 'pool backed security instrument' as there is no common industry name for this common parent class, other than 'asset backed security'.""" ;
	dct:license "http://opensource.org/licenses/MIT"^^xsd:anyURI ;
	sm:contentLanguage "https://www.w3.org/TR/owl2-quick-reference/"^^xsd:anyURI ;
	sm:copyright "Copyright (c) 2015-2021 EDM Council, Inc." ;
	sm:dependsOn
		"https://spec.edmcouncil.org/fibo/ontology/FBC/"^^xsd:anyURI ,
		"https://spec.edmcouncil.org/fibo/ontology/FND/"^^xsd:anyURI ,
		"https://spec.edmcouncil.org/fibo/ontology/SEC/Debt/Bonds/"^^xsd:anyURI ,
		"https://spec.edmcouncil.org/fibo/ontology/SEC/Debt/DebtInstruments/"^^xsd:anyURI ,
		"https://spec.edmcouncil.org/fibo/ontology/SEC/Securities/Pools/"^^xsd:anyURI ,
		"https://spec.edmcouncil.org/fibo/ontology/SEC/Securities/SecuritiesIssuance/"^^xsd:anyURI
		;
	sm:fileAbbreviation "fibo-sec-dbt-ab-pbs" ;
	sm:filename "PoolBackedSecurities.rdf" ;
	owl:imports
		<https://spec.edmcouncil.org/fibo/ontology/master/latest/FBC/DebtAndEquities/Debt/> ,
		<https://spec.edmcouncil.org/fibo/ontology/master/latest/FBC/FinancialInstruments/FinancialInstruments/> ,
		<https://spec.edmcouncil.org/fibo/ontology/master/latest/FND/Accounting/AccountingEquity/> ,
		<https://spec.edmcouncil.org/fibo/ontology/master/latest/FND/Agreements/Contracts/> ,
		<https://spec.edmcouncil.org/fibo/ontology/master/latest/FND/Arrangements/Arrangements/> ,
		<https://spec.edmcouncil.org/fibo/ontology/master/latest/FND/Relations/Relations/> ,
		<https://spec.edmcouncil.org/fibo/ontology/master/latest/FND/Utilities/AnnotationVocabulary/> ,
		<https://spec.edmcouncil.org/fibo/ontology/master/latest/SEC/Debt/Bonds/> ,
		<https://spec.edmcouncil.org/fibo/ontology/master/latest/SEC/Debt/DebtInstruments/> ,
		<https://spec.edmcouncil.org/fibo/ontology/master/latest/SEC/Securities/Pools/> ,
		<https://spec.edmcouncil.org/fibo/ontology/master/latest/SEC/Securities/SecuritiesIssuance/>
		;
	owl:versionIRI <https://spec.edmcouncil.org/fibo/ontology/master/latest/SEC/Debt/AssetBackedSecurities/PoolBackedSecurities/> ;
	fibo-fnd-utl-av:hasMaturityLevel fibo-fnd-utl-av:Provisional ;
	.

fibo-sec-dbt-ab-pbs:CashStructuredFinanceInstrument
	a owl:Class ;
	rdfs:subClassOf
		fibo-sec-dbt-ab-pbs:StructuredFinanceInstrument ,
		[
			a owl:Restriction ;
			owl:onProperty fibo-sec-dbt-ab-pbs:isTrancheOf ;
			owl:someValuesFrom fibo-sec-dbt-ab-pbs:SecuritizedDebtPool ;
		]
		;
	rdfs:label "cash-structured finance instrument"@en ;
	rdfs:isDefinedBy <https://spec.edmcouncil.org/fibo/ontology/SEC/Debt/AssetBackedSecurities/PoolBackedSecurities/> ;
	skos:definition "A structured finance instrument with a real asset underlying."@en ;
	.

fibo-sec-dbt-ab-pbs:CashStructuredFinanceInstrumentPool
	a owl:Class ;
	rdfs:subClassOf fibo-sec-dbt-ab-pbs:StructuredFinanceInstrumentPool ;
	rdfs:label "cash-structured finance instrument pool"@en ;
	rdfs:isDefinedBy <https://spec.edmcouncil.org/fibo/ontology/SEC/Debt/AssetBackedSecurities/PoolBackedSecurities/> ;
	skos:definition "A pool investment consisting of a collection of cash structured finance instruments."@en ;
	.

fibo-sec-dbt-ab-pbs:CollateralizedDebt
	a owl:Class ;
	rdfs:subClassOf
		fibo-sec-dbt-dbti:PubliclyIssuedDebt ,
		[
			a owl:Restriction ;
			owl:onProperty fibo-fbc-dae-dbt:isCollateralizedBy ;
			owl:someValuesFrom fibo-fnd-acc-aeq:FinancialAsset ;
		]
		;
	rdfs:label "collateralized debt"@en ;
	rdfs:isDefinedBy <https://spec.edmcouncil.org/fibo/ontology/SEC/Debt/AssetBackedSecurities/PoolBackedSecurities/> ;
	skos:definition "Debt issued under some Security, with some Collateral."@en ;
	.

fibo-sec-dbt-ab-pbs:CollateralizedObligationOffering
	a owl:Class ;
	rdfs:subClassOf fibo-sec-dbt-dbti:DebtOffering ;
	rdfs:label "collateralized obligation"@en ;
	rdfs:isDefinedBy <https://spec.edmcouncil.org/fibo/ontology/SEC/Debt/AssetBackedSecurities/PoolBackedSecurities/> ;
	skos:definition "Pending further investigation. At present: CDO = issued against pool of securities MBS = issued against pool of individual debts (base loans) Action: identify if this is the case. Option 1: Model as it was; Option 2: Add a level of detail in between, whereby there is a pool of pools or some other such thing Option 3: this is a terminological thing only in that CDOs are never referred to as a parent of CMO for purely teerminological reasons as per ABS v MBS in which case we would add in a terminological layer."@en ;
	.

fibo-sec-dbt-ab-pbs:PoolBackedDealProspectus
	a owl:Class ;
	rdfs:subClassOf fibo-sec-sec-iss:Prospectus ;
	rdfs:label "pool backed deal prospectus"@en ;
	rdfs:isDefinedBy <https://spec.edmcouncil.org/fibo/ontology/SEC/Debt/AssetBackedSecurities/PoolBackedSecurities/> ;
	skos:definition "Prospectus describing the terms of the issue and each of the instruments included in the pool backed security issue. Term origin:SMER"@en ;
	.

fibo-sec-dbt-ab-pbs:PoolBackedSecuritiesOffering
	a owl:Class ;
	rdfs:subClassOf
		fibo-sec-dbt-dbti:DebtOffering ,
		[
			a owl:Restriction ;
			owl:onProperty fibo-fnd-rel-rel:appliesTo ;
			owl:someValuesFrom fibo-sec-dbt-ab-pbs:PoolBackedSecurity ;
		] ,
		[
			a owl:Restriction ;
			owl:onProperty fibo-fnd-rel-rel:refersTo ;
			owl:someValuesFrom fibo-sec-dbt-ab-pbs:SecuritizedDebtPool ;
		]
		;
	rdfs:label "pool-backed securities offering"@en ;
	rdfs:isDefinedBy <https://spec.edmcouncil.org/fibo/ontology/SEC/Debt/AssetBackedSecurities/PoolBackedSecurities/> ;
	skos:definition "The issue of a series of Pool Backed Security certificates. These are (at least in this context) securities issued backed by a pool of individual loans, mortgages or other individual loan products."@en ;
	skos:editorialNote 'This term makes the distinction, perhaps artificial, between deals backed by pools of individual debt (this term), and deals backed by pools of securities (collateralized deals). This structure of relations between kinds of deals may prove to be a little artificial, but it reflects the structure of relations between kinds of securities, arrived at in earlier SME reviews. That is, Pool Backed Security (which breaks down into ABS and MBS) has a pool of individual loan products (a sub type of which is mortgage loans). The terms reflect the fact that in common parlance the term "ABS" is taken to mean something which is explicitly NOT a MBS but can be any other type of loan or credit based security, hence the creation of the non standard term "Pool Backed Security". The naming of deals simply attempts to reflect that. Terms to be included in Deal (per PoC conversations): Underwriters Issuer Deal Number Series number Deal Value Different collateral pools that support the deal. Review existing terms and make sure all covered.'@en ;
	.

fibo-sec-dbt-ab-pbs:PoolBackedSecurity
	a owl:Class ;
	rdfs:subClassOf
		fibo-sec-dbt-ab-pbs:StructuredFinanceInstrument ,
		[
			a owl:Restriction ;
			owl:onProperty fibo-fnd-agr-ctr:definesTermsFor ;
			owl:someValuesFrom fibo-sec-dbt-ab-pbs:CollateralizedDebt ;
		] ,
		[
			a owl:Restriction ;
			owl:onProperty fibo-sec-dbt-ab-pbs:isTrancheOf ;
			owl:someValuesFrom fibo-sec-sec-pls:DebtPool ;
		]
		;
	rdfs:label "pool-backed security"@en ;
	rdfs:isDefinedBy <https://spec.edmcouncil.org/fibo/ontology/SEC/Debt/AssetBackedSecurities/PoolBackedSecurities/> ;
	skos:definition "bond or note that derives its cashflow from some underlying pool of debt in which loans or mortgage advanced to borrowers are pooled together for the purposes of creating this type of security"@en ;
	.

fibo-sec-dbt-ab-pbs:SecuritizedDebtPool
	a owl:Class ;
	rdfs:subClassOf fibo-sec-sec-pls:DebtPool ;
	rdfs:label "securitized debt pool"@en ;
	rdfs:isDefinedBy <https://spec.edmcouncil.org/fibo/ontology/SEC/Debt/AssetBackedSecurities/PoolBackedSecurities/> ;
	skos:definition "pool of individual debt instruments (such as loans or mortgages) that is securitized as part of the issue of some security"@en ;
	.

fibo-sec-dbt-ab-pbs:StructuredFinanceInstrument
	a owl:Class ;
	rdfs:subClassOf fibo-sec-dbt-dbti:TradableDebtInstrument ;
	rdfs:label "structured finance instrument"@en ;
	rdfs:isDefinedBy <https://spec.edmcouncil.org/fibo/ontology/SEC/Debt/AssetBackedSecurities/PoolBackedSecurities/> ;
	skos:definition "debt instrument that has periodic principal payments with the amount of principal that is paid being dictated by a published factor"@en ;
	skos:example "Collateralized debt obligations (CDOs), synthetic financial instruments, collateralized bond obligations (CBOs), and syndicated loans are examples of structured finance instruments."@en ;
	fibo-fnd-utl-av:explanatoryNote "This may be either an invented product (synthetic) or based on a real underlying asset pool. Either way, the underlying is defined by the issuing bank or investment company. These are traded. This is based on tranches of underlying asset pools. These are defined by the issuing bank or investment company."@en ;
	.

fibo-sec-dbt-ab-pbs:StructuredFinanceInstrumentPool
	a owl:Class ;
	rdfs:subClassOf
		fibo-sec-sec-pls:InstrumentPool ,
		[
			a owl:Restriction ;
			owl:onProperty fibo-fnd-arr-arr:hasConstituent ;
			owl:someValuesFrom fibo-sec-dbt-ab-pbs:StructuredFinanceInstrument ;
		]
		;
	rdfs:label "structured finance instrument pool"@en ;
	rdfs:isDefinedBy <https://spec.edmcouncil.org/fibo/ontology/SEC/Debt/AssetBackedSecurities/PoolBackedSecurities/> ;
	skos:definition "pool consisting of a collection of structured finance instruments"@en ;
	.

fibo-sec-dbt-ab-pbs:backs
	a owl:ObjectProperty ;
	rdfs:label "backs"@en ;
	rdfs:domain fibo-sec-dbt-ab-pbs:SecuritizedDebtPool ;
	rdfs:isDefinedBy <https://spec.edmcouncil.org/fibo/ontology/SEC/Debt/AssetBackedSecurities/PoolBackedSecurities/> ;
	rdfs:range fibo-sec-dbt-ab-pbs:CashStructuredFinanceInstrument ;
	owl:inverseOf fibo-sec-dbt-ab-pbs:isTrancheOf ;
	.

fibo-sec-dbt-ab-pbs:isTrancheOf
	a owl:ObjectProperty ;
	rdfs:label "is tranche of"@en ;
	rdfs:domain fibo-sec-dbt-ab-pbs:CashStructuredFinanceInstrument ;
	rdfs:isDefinedBy <https://spec.edmcouncil.org/fibo/ontology/SEC/Debt/AssetBackedSecurities/PoolBackedSecurities/> ;
	rdfs:range fibo-sec-dbt-ab-pbs:SecuritizedDebtPool ;
	skos:definition "The asset pool which is the underlying of a traditional or cash structured finance instrument. This is a real pool of real assets, as distinct from synthetic pools."@en ;
	.

fibo-sec-dbt-ab-pbs:passThrough
	a owl:DatatypeProperty ;
	rdfs:label "pass through"@en ;
	rdfs:domain fibo-sec-dbt-ab-pbs:CashStructuredFinanceInstrument ;
	rdfs:isDefinedBy <https://spec.edmcouncil.org/fibo/ontology/SEC/Debt/AssetBackedSecurities/PoolBackedSecurities/> ;
	rdfs:range xsd:boolean ;
	skos:definition "Whether the cash flows from the underlying asset pool are passed through to the investor by way of redemption payments."@en ;
	.

fibo-sec-sec-pls:DebtPool
	a owl:Class ;
	rdfs:subClassOf [
		a owl:Restriction ;
		owl:onProperty fibo-sec-dbt-ab-pbs:backs ;
		owl:someValuesFrom fibo-sec-dbt-ab-pbs:PoolBackedSecurity ;
	] ;
	.

